Small changes to formatting

theories/stdpp_restrict.v
@@ -2,32 +2,32 @@ From Coq Require Import ssreflect.
 From stdpp Require Import fin_maps fin_map_dom.
 
 Definition restrict {K M} `{FinMap K M}
-  {D} (P: K -> D -> Prop) s `{∀ k, Decision (P k s)}
+  {D} (P: K → D → Prop) s `{∀ k, Decision (P k s)}
   {A} (m: M A) :=
-  filter (fun '(k,_) => P k s) m.
+  filter (λ '(k,_), P k s) m.
 
 Section restrict.
   Context {K M} `{FinMap K M}.
 
   Section simple_facts.
-    Context {D} (P: K -> D -> Prop) s `{∀ k, Decision (P k s)}.
-    Context {A:Type}.
-    Implicit Types (m : M A) (v:A).
+    Context {D} (P : K → D → Prop) s `{∀ k, Decision (P k s)}.
+    Context {A : Type}.
+    Implicit Types (m : M A) (v : A).
 
     (* In case we feel another definition would be better *)
-    Lemma restrict_filter m: restrict P s m = filter (fun '(k,_) => P k s) m.
+    Lemma restrict_filter m : restrict P s m = filter (λ '(k,_), P k s) m.
     Proof. reflexivity. Qed.
 
-    Lemma restrict_lookup_Some m k v:
-      restrict P s m !! k = Some v <-> m !! k = Some v /\ P k s.
+    Lemma restrict_lookup_Some m k v :
+      restrict P s m !! k = Some v ↔ m !! k = Some v ∧ P k s.
     Proof. apply map_filter_lookup_Some. Qed.
 
-    Lemma restrict_lookup_Some_2 m k v:
-      m !! k = Some v -> P k s -> restrict P s m !! k = Some v.
+    Lemma restrict_lookup_Some_2 m k v :
+      m !! k = Some v → P k s → restrict P s m !! k = Some v.
     Proof. intros. rewrite restrict_lookup_Some. done. Qed.
 
-    Lemma restrict_lookup_None m k:
-      restrict P s m !! k = None <-> m !! k = None \/ ¬ P k s.
+    Lemma restrict_lookup_None m k :
+      restrict P s m !! k = None ↔ m !! k = None ∨ ¬ P k s.
     Proof.
       split. intros Hr.
       destruct (m!!k) eqn:Hm.
@@ -42,12 +42,12 @@ Section restrict.
         contradiction (Hp' Hp).
     Qed.
 
-    Lemma restrict_lookup_None_2l m k:
-      m !! k = None -> restrict P s m !! k = None.
+    Lemma restrict_lookup_None_2l m k :
+      m !! k = None → restrict P s m !! k = None.
     Proof. intros. rewrite restrict_lookup_None. left. done. Qed.
 
-    Lemma restrict_lookup_None_2r m k:
-      ¬ P k s -> restrict P s m !! k = None.
+    Lemma restrict_lookup_None_2r m k :
+      ¬ P k s → restrict P s m !! k = None.
     Proof. intros. rewrite restrict_lookup_None. right. done. Qed.
 
     Lemma restrict_subseteq m: restrict P s m ⊆ m.
@@ -55,11 +55,11 @@ Section restrict.
 
     Lemma dom_restrict_subseteq m
       `{∀ A : Type, Dom (M A) D, ElemOf K D, Empty D, Singleton K D,
-      Union D, Intersection D, Difference D, !FinMapDom K M D}:
+      Union D, Intersection D, Difference D, !FinMapDom K M D} :
       dom (restrict P s m) ⊆ dom m.
     Proof. apply subseteq_dom, restrict_subseteq. Qed.
 
-    Lemma restrict_lookup m k:
+    Lemma restrict_lookup m k :
       restrict P s m !! k = (m !! k) ≫= λ v,
       match decide (P k s) with
         |left _ => Some v
@@ -79,26 +79,26 @@ Section restrict.
       apply restrict_lookup_None_2l, lookup_empty.
     Qed.
 
-    Lemma restrict_singleton k v:
+    Lemma restrict_singleton k v :
       restrict P s {[ k:=v ]} = match decide (P k s) with
       |left _ => {[ k:=v ]}
       |right _ => ∅
       end.
     Proof. apply map_filter_singleton. Qed.
 
-    Lemma restrict_union_complement m:
-      restrict P s m ∪ restrict (fun k s => ¬ P k s) s m = m.
+    Lemma restrict_union_complement m :
+      restrict P s m ∪ restrict (λ k s, ¬ P k s) s m = m.
     Proof. apply map_filter_union_complement. Qed.
 
-    Lemma restrict_empty_not_lookup m k:
-      restrict P s m = ∅ -> P k s -> m!!k = None.
+    Lemma restrict_empty_not_lookup m k :
+      restrict P s m = ∅ → P k s → m!!k = None.
     Proof.
       rewrite map_empty. setoid_rewrite restrict_lookup_None.
       intros Hi HP. destruct (Hi k) as [Hi'|Hi']. exact Hi'.
       contradiction (Hi' HP).
     Qed.
 
-    Lemma restrict_delete m i: restrict P s (delete i m) = delete i (restrict P s m).
+    Lemma restrict_delete m i : restrict P s (delete i m) = delete i (restrict P s m).
     Proof. apply map_filter_delete. Qed.
 
     Lemma restrict_fmap {B} (f : B → A) (m : M B) :
@@ -123,16 +123,16 @@ Section restrict.
   End simple_facts.
 
   Lemma restrict_restrict
-    {D1 D2} (P1: K -> D1 -> Prop) (P2: K -> D2 -> Prop) s1 s2
+    {D1 D2} (P1 : K → D1 → Prop) (P2 : K → D2 → Prop) s1 s2
     `{∀ s1 k, Decision (P1 k s1)} `{∀ s2 k, Decision (P2 k s2)}
-    {A} (m:M A):
-    restrict P1 s1 (restrict P2 s2 m) = restrict (fun k s => P1 k s1 /\ P2 k s2) (s1,s2) m.
+    {A} (m : M A) :
+    restrict P1 s1 (restrict P2 s2 m) = restrict (λ k s, P1 k s1 ∧ P2 k s2) (s1,s2) m.
   Proof. apply map_filter_filter. Qed.
 
   Lemma restrict_restrict_comm
-    {D1 D2} (P1: K -> D1 -> Prop) (P2: K -> D2 -> Prop) s1 s2
+    {D1 D2} (P1 : K → D1 → Prop) (P2 : K → D2 → Prop) s1 s2
     `{∀ s1 k, Decision (P1 k s1)} `{∀ s2 k, Decision (P2 k s2)}
-    {A} (m:M A):
+    {A} (m : M A) :
     restrict P1 s1 (restrict P2 s2 m) = restrict P2 s2 (restrict P1 s1 m).
   Proof.
     rewrite !restrict_restrict.
@@ -140,8 +140,8 @@ Section restrict.
   Qed.
 
   Lemma restrict_merge
-    {D} (P: K -> D -> Prop) s `{∀ k, Decision (P k s)}
-    {A B C} ml mr (f: option A -> option B -> option C) :
+    {D} (P: K → D → Prop) s `{∀ k, Decision (P k s)}
+    {A B C} ml mr (f: option A → option B → option C) :
     restrict P s (merge f ml mr) =
     merge f (restrict P s ml) (restrict P s mr).
   Proof.
@@ -155,14 +155,14 @@ Section restrict.
   Qed.
 
   Lemma restrict_map_zip_with
-    {D} (P: K -> D -> Prop) s `{∀ k, Decision (P k s)}
-    {A B C} ml mr (f: A -> B -> C) :
+    {D} (P: K → D → Prop) s `{∀ k, Decision (P k s)}
+    {A B C} ml mr (f: A → B → C) :
     restrict P s (map_zip_with f ml mr) =
     map_zip_with f (restrict P s ml) (restrict P s mr).
   Proof. apply restrict_merge. Qed.
 
   Lemma restrict_difference {A} (s:M A) (m:M A) :
-    restrict (fun k s => s!!k=None) s m = m ∖ s.
+    restrict (λ k s, s!!k = None) s m = m ∖ s.
   Proof.
     apply map_eq. intros k.
     rewrite restrict_lookup.
@@ -176,12 +176,12 @@ Section restrict.
   Section restrict_set.
     Context `{ElemOf K D, !RelDecision (∈@{D})}.
 
-    Definition restrict_set (s:D) {A} (m:M A) := restrict (∈) s m.
+    Definition restrict_set (s : D) {A} (m : M A) := restrict (∈) s m.
 
     Lemma dom_restrict_set_subseteq
       `{∀ A : Type, Dom (M A) D, Empty D, Singleton K D,
         Union D, Intersection D, Difference D, !FinMapDom K M D}
-      {A} s (m:M A) :
+      {A} s (m : M A) :
       dom (restrict_set s m) ⊆ s.
     Proof.
       intros x Hx. apply elem_of_dom in Hx as [y Hx].
@@ -191,7 +191,7 @@ Section restrict.
     Lemma dom_restrict_set
       `{∀ A : Type, Dom (M A) D, Empty D, Singleton K D,
         Union D, Intersection D, Difference D, !FinMapDom K M D}
-      {A} s (m:M A) :
+      {A} s (m : M A) :
       dom (restrict_set s m) ≡@{D} s ∩ dom m.
     Proof.
       apply set_equiv. intros k.
@@ -205,13 +205,13 @@ Section restrict.
     Lemma dom_restrict_set_L `{!LeibnizEquiv D}
       `{∀ A : Type, Dom (M A) D, Empty D, Singleton K D,
         Union D, Intersection D, Difference D, !FinMapDom K M D}
-      {A} s (m:M A) :
+      {A} s (m : M A) :
       dom (restrict_set s m) = s ∩ dom m.
     Proof. unfold_leibniz. apply dom_restrict_set. Qed.
 
     Lemma restrict_set_restrict_set `{Empty D, Singleton K D,
       Union D, Intersection D, Difference D, !Set_ K D}
-      {A} s1 s2 (m:M A) :
+      {A} s1 s2 (m : M A) :
       restrict_set s1 (restrict_set s2 m) = restrict_set (s1 ∩ s2) m.
     Proof.
       unfold restrict_set.
@@ -222,31 +222,27 @@ Section restrict.
 
   (** Another common case: restrict to keys present in another map *)
   Section restrict_map.
-    Definition restrict_map {A B} (s:M A) (m:M B) :=
-      restrict (fun k s => is_Some(s!!k)) s m.
+    Definition restrict_map {A B} (s : M A) (m : M B) :=
+      restrict (λ k s, is_Some(s!!k)) s m.
 
     Global Instance restrict_idemp {A} : IdemP (=@{M A}) restrict_map.
-    Proof.
-      intros m. apply map_eq. intros k. destruct (m!!k) as [v|] eqn:Hm.
-      apply restrict_lookup_Some_2. apply Hm. exists v. apply Hm.
-      apply restrict_lookup_None_2l. apply Hm.
-    Qed.
+    Proof. intros m. apply map_filter_id. intros k v. done. Qed.
 
     Context `{∀ A : Type, Dom (M A) D, ElemOf K D, Empty D, Singleton K D,
       Union D, Intersection D, Difference D, !FinMapDom K M D, !RelDecision (∈@{D})}.
 
-    Lemma restrict_map_restrict_set {A B} (s:M A) (m:M B):
+    Lemma restrict_map_restrict_set {A B} (s : M A) (m : M B) :
       restrict_map s m = restrict_set (dom s) m.
     Proof. apply map_filter_ext. intros. rewrite elem_of_dom. reflexivity. Qed.
 
-    Lemma dom_restrict_map {A B} (s:M A) (m:M B):
+    Lemma dom_restrict_map {A B} (s : M A) (m : M B) :
       dom (restrict_map s m) ≡@{D} dom s ∩ dom m.
     Proof. rewrite restrict_map_restrict_set. apply dom_restrict_set. Qed.
     Lemma dom_restrict_map_L `{!LeibnizEquiv D} {A B} (s:M A) (m: M B) :
       dom (restrict_map s m) = dom s ∩ dom m.
     Proof. unfold_leibniz. apply dom_restrict_map. Qed.
 
-    Lemma dom_restrict_map_subseteq {A B} (s:M A) (m:M B):
+    Lemma dom_restrict_map_subseteq {A B} (s : M A) (m : M B) :
       dom (restrict_map s m) ⊆ dom s.
     Proof. rewrite restrict_map_restrict_set. apply dom_restrict_set_subseteq. Qed.
   End restrict_map.
@@ -254,7 +250,8 @@ End restrict.
 
 
 (** map_zip ignores keys that aren't shared by both maps *)
-Lemma map_zip_with_minimal {K M A B C} `{FinMapDom K M D, !RelDecision (∈@{D})} (m1: M A) (m2: M B) (f: A → B → C):
+Lemma map_zip_with_minimal {K M A B C} `{FinMapDom K M D, !RelDecision (∈@{D})}
+  (m1 : M A) (m2 : M B) (f : A → B → C) :
   map_zip_with f m1 m2 =
   map_zip_with f (restrict_map m2 m1) (restrict_map m1 m2).
 Proof.
